case_studies/minivec/output/minivec/proofs/proof_RawVec_T_grow.v
@@ -29,13 +29,6 @@ Proof.
     rewrite ly_size_mk_array_layout.
     clear. solve_goal with nia.
   }
-  {
-    revert select (ly_size (mk_array_layout _ _) ≤ _).
-    move: Hnot_sz.
-    match goal with H : 2 * MaxInt ISize < MaxInt USize |- _ => move: H end.
-    rewrite ly_size_mk_array_layout.
-    solve_goal with nia.
-  }
 
   Unshelve. all: print_remaining_sidecond.
 Qed.
