theories/lithium/hooks.v
@@ -49,11 +49,15 @@ Ltac after_intro_hook H := idtac.
 (** [before_revert_hook H] is executed before reverting a pure Coq assumption [H]. *)
 Ltac before_revert_hook H := idtac.
 
-(** [shelve_sidecond_hook] is executed before shelving a sidecondition *)
-Ltac shelve_sidecond_hook := idtac.
-
 (** [liSidecond_hook] is executed before examining a pure Coq sidecondition [P] *)
 Ltac liSidecond_hook P := idtac.
+
+(** [liAfterSidecond_hook] is executed after processing a pure Coq sidecondition [P], 
+  but before splitting the goal for shelving. *)
+Ltac liAfterSidecond_hook P := idtac.
+
+(** [shelve_sidecond_hook] is executed before shelving a sidecondition *)
+Ltac shelve_sidecond_hook := idtac.
 
 (** [generate_i2p_instance_to_tc_hook] is used to infer the
 typeclasses from the lemmas for the [instance] notation for declaring
